Make functions opaque and documentation. see #32

src/dafny/utils/EVMObject.dfy
@@ -13,6 +13,7 @@
  */
 
 include "../utils/LinSegments.dfy"
+include "../utils/CFGState.dfy"
 include "../utils/State.dfy"
 include "../utils/MiscTypes.dfy"
 include "../utils/Instructions.dfy"
@@ -32,6 +33,7 @@ include "../CFGBuilder/BuildCFGSimplified.dfy"
 module EVMObject {
 
   import opened LinSegments
+  import opened CFGState
   import opened State
   import opened MiscTypes
   import Instructions
@@ -42,22 +44,31 @@ module EVMObject {
   import opened DFSSimple
   import opened PartitionMod
   import opened AStateMinimiser
+  import opened WeakPre
+  import opened StackElement
 
+  /**
+    *    A valid sequence of valid linear segments. To be valid the sequence 
+    *    must be ordered by start addresses.
+    */
+  type ValidSeqValidLinSeg = xs: seq<ValidLinSeg> | forall i, i':: 0 <= i < i' < |xs| ==> xs[i].StartAddress() < xs[i'].StartAddress()
 
-  /**   A valid EVMObj should have jumpdests consistent with the segments. */
-  type ValidEVMObj = e: EVMObj | e.jumpDests == CollectJumpDests(e.xs)
-    witness EVMObj([], [])
+  /**   A valid EVMObj should have a PCToSegMap that is the reverse of xs -> startAddress() . */
+  type ValidEVMObj = e: EVMObj | e.IsValid() witness EVMObj([], [])
 
   /**   An EVMObj has segments and jumpDests. */
   datatype EVMObj = EVMObj(
-    xs: seq<ValidLinSeg>,
-    jumpDests: seq<nat> := CollectJumpDests(xs)) {
+    xs: ValidSeqValidLinSeg,
+    jumpDests: seq<nat> := CollectJumpDests(xs),
+    startAddresses: seq<nat> := CollectStartAddresses(xs),
+    PCToSegMap: map<nat, nat> := CollectThem(xs)
+    // PCToSegMap: map<nat, nat> := CollectPCToSeg(xs) . does not work with VsCode plugin ...hangs up
+  ) {
 
     /** A valid EVMObj has jumpDests consistent with xs. */
     predicate IsValid() {
       && (forall i, i':: 0 <= i < i' < |xs| ==> xs[i].StartAddress() < xs[i'].StartAddress())
-    //   && jumpDests == CollectJumpDests(xs)
-    //   && startAddresses == CollectStartAddresses(xs)
+      && (forall k:: k in PCToSegMap ==> PCToSegMap[k] < |xs| && xs[PCToSegMap[k]].StartAddress() == k)
     }
 
     /** The size of the program in bytes. */
@@ -66,19 +77,174 @@ module EVMObject {
       else ls[0].Size() + Size(ls[1..])
     }
 
+    // lemma foo101(s: ValidLinSeg, c:seq<nat>)
+    //   requires |c| <= s.NumberOfExits()
+    //   ensures forall k {:nowarn}:: 0 <= k < |c| ==> k < s.NumberOfExits()
+    //   ensures forall k:: 0 <= k < |c| ==> s.IsValidExit(k)
+    // {   //  Thanks Dafny
+    // }
+
     /**
       * Compute the next abstract states from a given abstract state.
+      * @param s The abstract state.
+      * @returns The next abstract states.
+      *
+      * @note   This function is _inductive_ in the sense of the Inductive predicate (see BuildCFG).
       */
-    function Next(s: AState): seq<AState>
+    function {:opaque} NextG(s: GState): (r: seq<GState>)
+      requires this.IsValid()
+      requires s.EGState? ==> s.segNum < |xs|
+      ensures forall k:: 0 <= k < |r| && r[k].EGState? ==> r[k].segNum < |xs|
     {
-      if s.Error? then []
-      else
-        match PCToSeg(s.pc) {
-          case Some(s0) =>
-            seq(xs[s0].NumberOfExits(), i requires 0 <= i < xs[s0].NumberOfExits() => xs[s0].Run(s, i, jumpDests))
-          case None => []
-        }
+      match s
+      case ErrorGState(_) => []
+      case EGState(segNum, st) =>
+        // compute next state
+        var srcSeg := xs[segNum];
+        var src: AState := EState(srcSeg.StartAddress(), st);
+        var successors := seq(srcSeg.NumberOfExits(), (i: nat) requires srcSeg.IsValidExit(i) => srcSeg.Run(src, i, jumpDests));
+        //  map to GState when PCToSegMap is defined
+        var succGStates :=
+          Map(
+            successors,
+            (s': AState) =>
+              match s'
+              case Error(msg) => ErrorGState(msg)
+              case EState(pc, st) =>
+                if pc in PCToSegMap then
+                  EGState(PCToSegMap[pc], s'.stack)
+                else
+                  ErrorGState("NextG:  " + Int.NatToString(pc) + " not defined")
+          );
+        succGStates
     }
+
+    /**   Execute a sequence of segments.
+      *
+      *   @param  exist       Exists after each segment.
+      *   @param  s           A state.
+      *
+      */
+    function {:opaque} RunAll(exits: seq<nat>, s: AState): AState
+      requires this.IsValid()
+      requires s.EState?
+    {
+      if |exits| == 0 then s
+      else match PCToSeg(s.pc)
+           case Some(seg) =>
+             if xs[seg].NumberOfExits() > exits[0] then
+               foo(xs[seg], exits[0]);
+               var s' := xs[seg].Run(s, exits[0], jumpDests);
+               if s'.EState? then
+                 // Run the rest of the path
+                 RunAll(exits[1..], s')
+               else
+                 //  exit does not exist, return the error state.
+                 Error("Successor state of " + s.ToString() + " is not an EState")
+             else
+               //  exit does not exist
+               Error("Exit does not exist")
+           case None => Error("No segment found for state " + s.ToString())
+
+    }
+
+    /**
+      *   Whether a condition is invariant under a given path.
+      *   @param  c           A condition.
+      *   @param  exits       The exit after each segment.
+      */
+    predicate {:opaque} PreservesCond(c: ValidCond, exits: seq<nat>)
+      requires this.IsValid()
+      requires c.StCond?
+    {
+      var initState := BuildInitState(c);
+      var endState := RunAll(exits, initState);
+      if endState.EState? then
+        endState.Sat(c)
+      else false
+    }
+
+    /**
+      *   Check if a state whit this pc has been seen before, and whether we can loop back 
+      *   to an already seen state on this path.
+      *
+      *   @note   The seenOnPath has all the nodes seen before the current one.
+      *           The current one has startAddress == pc.
+      */
+    // function SafeLoopFound(pc: nat, seenOnPath: seq<AState>, exits: seq<nat>): (r: Option<AState>)
+    //   requires this.IsValid()
+    //   requires |xs| >= 1
+    //   requires pc < Int.TWO_256
+    //   requires 0 < |seenOnPath| // == |path|
+    //   requires |exits| == |seenOnPath|
+    //   requires forall k :: 0 <= k < |seenOnPath| ==> seenOnPath[k].EState? && PCToSeg(seenOnPath[k].pc).Some?
+    //   // requires forall k:: k in seenOnPath ==> k.seg.Some? && k.seg.v < |xs|
+    //   // requires xs[seenOnPath[|seenOnPath| - 1].seg.v].JUMPSeg? || xs[seenOnPath[|seenOnPath| - 1].seg.v].JUMPISeg?
+    //   // ensures r.Some? ==> r.v.seg.Some? && r.v.seg.v < |xs|
+    //   decreases |seenOnPath|
+    // {
+    //   match FindFirstNodeWithPC(pc, seenOnPath)
+    //   case Some(v) =>
+    //     //  pc occurs on this path and v is an abstract state s with s.pc == pc
+    //     assert v.0.EState?;
+    //     assert v.0.pc == pc;
+    //     //  some properties must hold on the path defined by the index v.1
+    //     var init := seenOnPath[v.1];
+    //     //  the CFGMNode at index v.1 has a segment with start address == pc
+    //     //   assert xs[init.seg.v].StartAddress() == pc;
+    //     //  get the path false|true that led from init to last node
+    //     var path := seenOnPath[v.1..];
+    //     //   //  compute the list of segments defined by the nodes in path
+    //     //   var segs := NodesToSeg(path);
+    //     assert forall k :: 0 <= k < |path| ==> path[k].EState? && PCToSeg(path[k].pc).Some?;
+    //     var segs := seq(|path|, i requires 0 <= i < |path| => PCToSeg(path[i].pc).v);
+    //     //  compute the Wpre for last node path to lead to pc (via true)
+    //     assert pc < Int.TWO_256;
+    //     assume xs[PCToSeg(seenOnPath[|seenOnPath| - 1].pc).v].IsValidExit(exits[|exits| - 1]);
+    //     var tgtCond := xs[PCToSeg(seenOnPath[|seenOnPath| - 1].pc).v].LeadsTo(pc, exits[|exits| - 1]);
+    //     //    Compute the WPre for for segments in path
+    //     var w1 := WPreSeqSegs(segs, exits[v.1..], tgtCond, xs, pc);
+    //     //   if w1.StTrue? then
+    //     //     Some(v.0)
+    //     //   else if w1.StFalse? then
+    //     //     None
+    //     //   else if PreservesCond(w1, segs, boolPath[v.1..], xs, jumpDests) then
+    //     //     Some(v.0)
+    //     //   //  Try a potential second occurrence of pc om seenOnPath
+    //     //   else if 0 < |seenOnPath[v.1..|seenOnPath|]| < |seenOnPath| then
+    //     //     SafeLoopFound(xs, pc, seenOnPath[v.1..|seenOnPath|], boolPath[v.1..|boolPath|], jumpDests)
+    //     //   else None
+    //     None
+
+    //   case None =>
+    //     //  No occurrence of pc on this path
+    //     None
+    // }
+
+    /**
+      *   Find the first node in a sequence with a givem value for pc.
+      *   @param  pc      The pc to find in s.
+      *   @param  s       A sequence of states.
+      *   @param  index   The current index in the search.
+      *   @returns        The node, index of the first occurrence of a state in s with 
+      *                   s.pc equals to pc. 
+      */
+    // function FindFirstNodeWithPC(pc: nat, s: seq<AState>, index: nat := 0): (r: Option<(AState, nat)>)
+    //   requires index <= |s|
+    //   ensures r.Some? ==> r.v.0.EState?
+    //   ensures r.Some? ==> r.v.1 < |s|
+    //   ensures r.Some? ==> s[r.v.1].EState?
+    //   ensures r.Some? ==> s[r.v.1].pc == pc == r.v.0.pc
+    //   decreases |s| - index
+    // {
+    //   if |s| == index then None
+    //   else
+    //     match s[index]
+    //     case EState(pc', st) =>
+    //       if pc' == pc then Some((s[index], index))
+    //       else FindFirstNodeWithPC(pc, s, index + 1)
+    //     case Error(m) => None
+    // }
 
     /**
       * Build the CFG of the EVMObj.
@@ -86,13 +252,17 @@ module EVMObject {
       * @param maxDepth The maximum depth of the DFS.
       * @param minimise If true, the CFG is minimised.   
       */
-    method BuildCFG(maxDepth: nat := 100, minimise: bool := true) returns (a: Automata.ValidAuto<AState>)
+    method {:opaque} BuildCFG(maxDepth: nat := 100, minimise: bool := true) returns (a: Automata.ValidAuto<GState>)
+      requires this.IsValid()
+      requires |xs| >= 1
+      ensures forall s:: s in a.states && s.EGState? ==> s.segNum < |xs|
     {
       //  For now we ignore the history
       var a1, _ := DFS(
-        Next,
-        DEFAULT_VALIDSTATE,
-        History(DEFAULT_VALIDSTATE, [DEFAULT_VALIDSTATE]),
+        NextG,
+        // DEFAULT_VALIDSTATE,
+        DEFAULT_GSTATE,
+        History(DEFAULT_GSTATE, [DEFAULT_GSTATE]),
         Automata.Auto(),
         maxDepth);
       if !minimise || a1.SSize() == 0 {
@@ -106,7 +276,7 @@ module EVMObject {
               true
             else
               match (a1.states[x], a1.states[y])
-              case (EState(pc1,_), EState(pc2, _)) => PCToSeg(pc1).Some? && PCToSeg(pc2).Some? && pc1 == pc2
+              case (EGState(s1,_), EGState(s2, _)) => s1 == s2
               case (_, _) => false
           ;
         assert IsEquivRel(e, a1.SSize());
@@ -119,33 +289,84 @@ module EVMObject {
 
     }
 
+    // lemma foo303()
+    //   requires this.IsValid()
+    //   requires |xs| >= 1
+    //   ensures NextG.requires(DEFAULT_GSTATE)
+    // { assert NextG.requires(DEFAULT_GSTATE); }
+
     /**
-      * Generate the HTNL representation of a given abstract state.
+      * Generate the HTML representation of a given abstract state.
       */
-    function ToHTML(a: AState): string {
-      if a.Error? then
+    function ToHTML(a: GState): string
+      requires this.IsValid()
+      requires a.EGState? ==> a.segNum < |xs|
+    {
+      if a.ErrorGState? then
         "<ErrorEnd <BR ALIGN=\"CENTER\"/>>"
       else
-        match PCToSeg(a.pc) {
-          case Some(seg1) =>
-            "<" + DOTSeg(xs[seg1], seg1).0 +">"
-          case None =>  "<ErrorEnd <BR ALIGN=\"CENTER\"/>>"
-        }
+        //  because of the pre-condition, we are sure that a has a segNum < |xs|
+        //  and we can use xs[a.segNum]
+        "<" + DOTSeg(xs[a.segNum], a.segNum).0 +">"
     }
 
     /**
       *   Retrieve num of segment that correspond to a PC if any.
       */
-    function PCToSeg(pc: nat, rank: nat := 0): (r: Option<nat>)
-      requires rank <= |xs|
-      ensures r.Some? ==> r.v < |xs|
-      ensures r.Some?  ==> xs[r.v].StartAddress() == pc
-      decreases |xs| - rank
+    // function PCToSeg(pc: nat, rank: nat := 0): (r: Option<nat>)
+    //   requires this.IsValid()
+    //   requires rank <= |xs|
+    //   ensures r.Some? ==> r.v < |xs|
+    //   ensures r.Some?  ==> xs[r.v].StartAddress() == pc
+    //   //   ensures pc in startAddresses ==> r.Some?
+    //   decreases |xs| - rank
+    // {
+    //   if rank == |xs| then None
+    //   else if xs[rank].StartAddress() == pc then Some(rank)
+    //   else PCToSeg(pc, rank + 1)
+    // }
+
+    function {:opaque} PCToSeg(pc: nat): (r: Option<nat>)
+      requires this.IsValid()
+      ensures r.Some? ==> r.v < |xs| && xs[r.v].StartAddress() == pc
     {
-      if rank == |xs| then None
-      else if xs[rank].StartAddress() == pc then Some(rank)
-      else PCToSeg(pc, rank + 1)
+      if pc in PCToSegMap then
+        Some(PCToSegMap[pc])
+      else
+        None
     }
+
+    // function CollectStartAddressOfSegs(): (r: seq<nat>)
+    //   ensures |xs| == |r|
+    // {
+    //   CollectStartAddresses(xs)
+    // }
+
+    // function CollectStartAddressesV2(index: nat := 0, m: map<nat, nat> := map[]): (r: map<nat, nat>)
+    //   requires index <= |xs|
+    //   requires |m| <= index <= |xs|
+    //   requires forall i:: 0 <= i < |m| ==> m[i] == xs[i].StartAddress()
+    //   ensures |r| <= |xs|
+    //   ensures forall i:: 0 <= i < |r| ==> r[i] == xs[i].StartAddress()
+    //   decreases |xs| - index
+    // {
+    //   if index == |xs| then m
+    //   else
+    //     // map[xs[index].StartAddress() := index] +
+    //     CollectStartAddressesV2(index + 1, m[xs[index].StartAddress() := index] )
+    // }
+
+    // lemma foo101(pc: nat)
+    //     requires pc in CollectStartAddressOfSegs()
+    //     // ensures PCToSeg(pc).Some?
+    // {
+    //     var k1 :| k1 in CollectStartAddressOfSegs() && k1 == pc;
+    //     var k :| 0 <= k < |CollectStartAddressOfSegs()| && CollectStartAddressOfSegs()[k] == pc;
+    //     assert 0 <= k < |xs|;
+    //     assert xs[k].StartAddress() == pc;
+    //     assert PCToSeg(pc).Some?;
+    // }
+
 
   }
 
@@ -177,12 +398,59 @@ module EVMObject {
   }
 
   /** Collect jumpdests in a list of segments.  */
-  function CollectJumpDests(xs: seq<ValidLinSeg>): seq<nat> {
+  function {:opaque} CollectJumpDests(xs: seq<ValidLinSeg>): seq<nat> {
     if |xs| == 0 then []
     else
       xs[0].CollectJumpDest() + CollectJumpDests(xs[1..])
   }
 
+  function {:opaque} CollectStartAddresses(segs: seq<ValidLinSeg>): (r: seq<nat>)
+    ensures |segs| == |r|
+    ensures forall i:: 0 <= i < |r| ==> r[i] == segs[i].StartAddress()
+  {
+    if |segs| == 0 then []
+    else
+      [segs[0].StartAddress()] + CollectStartAddresses(segs[1..])
+  }
+
+  /**
+    *  Collect the mapping from PC to segment number.
+    *  @note This is essentially the same as CollectPCToSeg but with less pre-conditions.
+    *        This function is called in the constructor of an EVMObj. 
+    *        The CollectPCToSeg causes the VsCode Dafny server to hang for ever.
+    *        When/if this bug is fixed we can use PCToSegMap in the constructor of EVMObj.
+    * @note  The CLI version of Dafny does not hang and verifies the code.
+    */
+  function {:opaque} CollectThem(xs: seq<ValidLinSeg>): (r: map<nat, nat>)
+    requires forall i, i':: 0 <= i < i' < |xs| ==> xs[i].StartAddress() < xs[i'].StartAddress()
+    ensures forall k:: 0 <= k < |xs| ==> xs[k].StartAddress() in r && r[xs[k].StartAddress()] == k
+    ensures forall k:: k in r ==> r[k] < |xs| && xs[r[k]].StartAddress() == k
+  {
+    CollectPCToSeg(xs)
+  }
+
+  /** 
+    *  Collect the mapping from PC to segment number.
+    *  @param  xs      A list of segments.
+    *  @param  m       The map that has been built so far. 
+    *  @param  index   The current index in the list of segments.
+    *  @returns        The map from PC to segment number.
+    *  @note           The resulkt satisfies some properties given by the ensures clauses.
+    */
+  function {:opaque} CollectPCToSeg(xs: seq<ValidLinSeg>, m: map<nat, nat> := map[], index: nat := 0): (r: map<nat, nat>)
+    requires index <= |xs|
+    requires forall i, i':: 0 <= i < i' < |xs| ==> xs[i].StartAddress() < xs[i'].StartAddress()
+    requires forall k:: 0 <= k < index ==> xs[k].StartAddress() in m
+    requires forall k:: 0 <= k < index ==> m[xs[k].StartAddress()] == k
+    requires forall k:: k in m ==> m[k] < |xs| && xs[m[k]].StartAddress() == k
+    ensures forall k:: 0 <= k < |xs| ==> xs[k].StartAddress() in r && r[xs[k].StartAddress()] == k
+    ensures forall k:: k in r ==> r[k] < |xs| && xs[r[k]].StartAddress() == k
+    decreases |xs| - index
+  {
+    if index == |xs| then m
+    else
+      CollectPCToSeg(xs, m[xs[index].StartAddress() := index], index + 1)
+  }
 
 }
 
